Added epoch to invariants; still need to update lemmas

ironfleet/src/Dafny/Distributed/Protocol/Lock/PerformanceProof/PerformanceProof.i.dfy
@@ -67,13 +67,13 @@ predicate PerfInvariantAlways(tgls:TaggedGLS_State)
   ==> pkt.msg.v.transfer_epoch <= |tgls.history|)
 }
 
-predicate {:opaque} PerfInvariantLockHeld(tgls: TaggedGLS_State, j:int)
+predicate {:opaque} PerfInvariantLockHeld(tgls: TaggedGLS_State, j:int, epoch:int)
   requires 0 <= j < |tgls.tls.config|
   requires TGLS_Consistency(tgls)
 {
     && PerfInvariantAlways(tgls)
     && tgls.tls.t_servers[tgls.tls.config[j]].v.held == true
-    && |tgls.history| == j + 1
+    && |tgls.history| == epoch + 1
     && tgls.tls.t_servers[tgls.tls.config[j]].v.epoch == |tgls.history|
 
     &&  (forall id :: id in tgls.tls.t_servers && id != tgls.tls.config[j]
@@ -105,40 +105,14 @@ predicate {:opaque} PerfInvariantLockHeld(tgls: TaggedGLS_State, j:int)
     )
 }
 
-predicate PerfInvariantLockHeldNonOpaque(tgls: TaggedGLS_State, j:int)
+predicate {:opaque} PerfInvariantLockInNetwork(tgls: TaggedGLS_State, j:int, epoch:int)
+  requires 0 <= epoch
   requires 0 <= j < |tgls.tls.config|
   requires TGLS_Consistency(tgls)
 {
-    && PerfInvariantAlways(tgls)
-    && tgls.tls.t_servers[tgls.tls.config[j]].v.held == true
-    && |tgls.history| == j + 1
-    && tgls.tls.t_servers[tgls.tls.config[j]].v.epoch == |tgls.history|
-
-    &&  (forall id :: id in tgls.tls.t_servers && id != tgls.tls.config[j]
-    ==> tgls.tls.t_servers[id].v.held == false && tgls.tls.t_servers[id].v.epoch < |tgls.history|)
-
-    // All packets have epoch too small, so that no packets can be accepted in the next step
-    && ( forall pkt :: pkt in tgls.tls.t_environment.sentPackets && pkt.msg.v.Transfer? && pkt.dst in tgls.tls.t_servers && pkt.src in tgls.tls.t_servers
-    ==> pkt.msg.v.transfer_epoch <= tgls.tls.t_servers[pkt.dst].v.epoch)
-
-    // The node with the lock has correct PerfReport
-    && PerfEq(tgls.tls.t_servers[tgls.tls.config[j]].pr, PerfBoundLockHeld(j))
-
-    // All nodes beyond j have void PerfReport
-    && (forall k :: j < k < |tgls.tls.config| ==> PerfEq(tgls.tls.t_servers[tgls.tls.config[k]].pr, PerfVoid()))
-
-    // No packets sent to nodes that have my_index higher than j
-    && (forall pkt, k :: j < k < |tgls.tls.config| && pkt in tgls.tls.t_environment.sentPackets && pkt.dst in tgls.tls.t_servers && pkt.dst == tgls.tls.config[k]
-    ==> false
-    )
-}
-
-predicate {:opaque} PerfInvariantLockInNetwork(tgls: TaggedGLS_State, j:int)
-  requires 0 < j < |tgls.tls.config|
-  requires TGLS_Consistency(tgls)
-{
   && PerfInvariantAlways(tgls)
-  && |tgls.history| == j + 1
+  && |tgls.history| == epoch + 1
+  && j == (epoch % |tgls.tls.config|)
 
   // No one holds the lock; everyone's epoch is below the epoch of the newest packet.
   && (forall id :: id in tgls.tls.t_servers ==> tgls.tls.t_servers[id].v.held == false && tgls.tls.t_servers[id].v.epoch < |tgls.history|)
@@ -149,7 +123,7 @@ predicate {:opaque} PerfInvariantLockInNetwork(tgls: TaggedGLS_State, j:int)
 
   && ( forall pkt :: pkt in tgls.tls.t_environment.sentPackets && pkt.msg.v.Transfer? && pkt.dst in tgls.tls.t_servers && pkt.src in tgls.tls.t_servers
       && pkt.msg.v.transfer_epoch == |tgls.history|
-      ==> pkt.dst == tgls.tls.config[j] && pkt.src == tgls.tls.config[j - 1] && PerfEq(pkt.msg.pr, PerfBoundLockInNetwork(j)))
+      ==> pkt.dst == tgls.tls.config[j] && pkt.src == tgls.tls.config[(j - 1) % |tgls.tls.config|] && PerfEq(pkt.msg.pr, PerfBoundLockInNetwork(j)))
 
   // All nodes beyond j have void PerfReport
   && (forall k :: j < k < |tgls.tls.config| ==> PerfEq(tgls.tls.t_servers[tgls.tls.config[k]].pr, PerfVoid()))
@@ -170,7 +144,7 @@ predicate {:opaque} PerfInvariantLockInNetwork(tgls: TaggedGLS_State, j:int)
   )
 }
 
-lemma NotHostIos_InvLockHeldImpliesInvLockHeld(j:int, s:TaggedGLS_State, s':TaggedGLS_State)
+lemma NotHostIos_InvLockHeldImpliesInvLockHeld(j:int, epoch:int, s:TaggedGLS_State, s':TaggedGLS_State)
   requires TGLS_Next(s, s')
   requires 0 <= j < |s.tls.config|
   requires TGLS_Consistency(s) && TGLS_Consistency(s')
@@ -178,13 +152,13 @@ lemma NotHostIos_InvLockHeldImpliesInvLockHeld(j:int, s:TaggedGLS_State, s':Tagg
   // Not a HostIos step
   requires !s.tls.t_environment.nextStep.LEnvStepHostIos?
 
-  requires PerfInvariantLockHeld(s, j);
-  ensures PerfInvariantLockHeld(s', j);
+  requires PerfInvariantLockHeld(s, j, epoch);
+  ensures PerfInvariantLockHeld(s', j, epoch);
 {
   reveal_PerfInvariantLockHeld();
 }
 
-lemma Grant_not_j_InvLockHeldImpliesInvLockHeld(j:int, s:TaggedGLS_State, s':TaggedGLS_State)
+lemma Grant_not_j_InvLockHeldImpliesInvLockHeld(j:int, epoch:int, s:TaggedGLS_State, s':TaggedGLS_State)
   requires TGLS_Next(s, s')
   requires 0 <= j < |s.tls.config|
   requires TGLS_Consistency(s) && TGLS_Consistency(s')
@@ -195,13 +169,13 @@ lemma Grant_not_j_InvLockHeldImpliesInvLockHeld(j:int, s:TaggedGLS_State, s':Tag
   requires s.tls.t_environment.nextStep.actor != s.tls.config[j]
   requires s.tls.t_environment.nextStep.nodeStep == GrantStep
 
-  requires PerfInvariantLockHeld(s, j);
-  ensures PerfInvariantLockHeld(s', j);
+  requires PerfInvariantLockHeld(s, j, epoch);
+  ensures PerfInvariantLockHeld(s', j, epoch);
 {
   reveal_PerfInvariantLockHeld();
 }
 
-lemma Accept_not_j_InvLockHeldImpliesInvLockHeld(j:int, s:TaggedGLS_State, s':TaggedGLS_State)
+lemma Accept_not_j_InvLockHeldImpliesInvLockHeld(j:int, epoch:int, s:TaggedGLS_State, s':TaggedGLS_State)
   requires TGLS_Next(s, s')
   requires 0 <= j < |s.tls.config|
   requires TGLS_Consistency(s) && TGLS_Consistency(s')
@@ -212,13 +186,13 @@ lemma Accept_not_j_InvLockHeldImpliesInvLockHeld(j:int, s:TaggedGLS_State, s':Ta
   requires s.tls.t_environment.nextStep.actor != s.tls.config[j]
   requires s.tls.t_environment.nextStep.nodeStep == AcceptStep
 
-  requires PerfInvariantLockHeld(s, j);
-  ensures PerfInvariantLockHeld(s', j);
+  requires PerfInvariantLockHeld(s, j, epoch);
+  ensures PerfInvariantLockHeld(s', j, epoch);
 {
   reveal_PerfInvariantLockHeld();
 }
 
-lemma Grant_j_InvLockHeldImpliesInvLockInNetwork(j:int, s:TaggedGLS_State, s':TaggedGLS_State)
+lemma Grant_j_InvLockHeldImpliesInvLockInNetwork(j:int, epoch:int, s:TaggedGLS_State, s':TaggedGLS_State)
   requires TGLS_Next(s, s')
   requires 0 <= j < |s.tls.config| - 1
   requires TGLS_Consistency(s) && TGLS_Consistency(s')
@@ -230,8 +204,8 @@ lemma Grant_j_InvLockHeldImpliesInvLockInNetwork(j:int, s:TaggedGLS_State, s':Ta
   requires s.tls.t_environment.nextStep.actor == s.tls.config[j]
   requires s.tls.t_environment.nextStep.nodeStep == GrantStep
 
-  requires PerfInvariantLockHeld(s, j);
-  ensures PerfInvariantLockInNetwork(s', j + 1);
+  requires PerfInvariantLockHeld(s, j, epoch);
+  ensures PerfInvariantLockInNetwork(s', j, epoch + 1);
 {
   reveal_PerfInvariantLockHeld();
   reveal_PerfInvariantLockInNetwork();
@@ -243,7 +217,7 @@ lemma Grant_j_InvLockHeldImpliesInvLockInNetwork(j:int, s:TaggedGLS_State, s':Ta
   assert PerfEq(p', PerfAdd2(p, PerfStep(GrantStep)));
 }
 
-lemma NotHostIos_InvLockInNetworkImpliesInvLockInNetwork(j:int, s:TaggedGLS_State, s':TaggedGLS_State)
+lemma NotHostIos_InvLockInNetworkImpliesInvLockInNetwork(j:int, epoch:int, s:TaggedGLS_State, s':TaggedGLS_State)
   requires TGLS_Next(s, s')
   requires 0 < j < |s.tls.config|
   requires TGLS_Consistency(s) && TGLS_Consistency(s')
@@ -251,13 +225,13 @@ lemma NotHostIos_InvLockInNetworkImpliesInvLockInNetwork(j:int, s:TaggedGLS_Stat
   // Not a HostIos step
   requires !s.tls.t_environment.nextStep.LEnvStepHostIos?
 
-  requires PerfInvariantLockInNetwork(s, j);
-  ensures PerfInvariantLockInNetwork(s', j);
+  requires PerfInvariantLockInNetwork(s, j, epoch);
+  ensures PerfInvariantLockInNetwork(s', j, epoch);
 {
   reveal_PerfInvariantLockInNetwork();
 }
 
-lemma Accept_not_j_InvLockInNetworkImpliesInvLockInNetwork(j:int, s:TaggedGLS_State, s':TaggedGLS_State)
+lemma Accept_not_j_InvLockInNetworkImpliesInvLockInNetwork(j:int, epoch:int, s:TaggedGLS_State, s':TaggedGLS_State)
   requires TGLS_Next(s, s')
   requires 0 < j < |s.tls.config| - 1
   requires TGLS_Consistency(s) && TGLS_Consistency(s')
@@ -269,15 +243,15 @@ lemma Accept_not_j_InvLockInNetworkImpliesInvLockInNetwork(j:int, s:TaggedGLS_St
   requires s.tls.t_environment.nextStep.actor != s.tls.config[j]
   requires s.tls.t_environment.nextStep.nodeStep == AcceptStep
 
-  requires PerfInvariantLockInNetwork(s, j);
-  ensures PerfInvariantLockInNetwork(s', j);
+  requires PerfInvariantLockInNetwork(s, j, epoch);
+  ensures PerfInvariantLockInNetwork(s', j, epoch);
 {
   reveal_PerfInvariantLockInNetwork();
 
   lemma_mod_auto(|s.tls.config|);
 }
 
-lemma Accept_j_InvLockInNetworkImpliesInvLockHeld(j:int, s:TaggedGLS_State, s':TaggedGLS_State)
+lemma Accept_j_InvLockInNetworkImpliesInvLockHeld(j:int, epoch:int, s:TaggedGLS_State, s':TaggedGLS_State)
   requires TGLS_Next(s, s')
   requires 0 < j < |s.tls.config| - 1
   requires TGLS_Consistency(s) && TGLS_Consistency(s')
@@ -289,8 +263,8 @@ lemma Accept_j_InvLockInNetworkImpliesInvLockHeld(j:int, s:TaggedGLS_State, s':T
   requires s.tls.t_environment.nextStep.actor == s.tls.config[j]
   requires s.tls.t_environment.nextStep.nodeStep == AcceptStep
 
-  requires PerfInvariantLockInNetwork(s, j);
-  ensures PerfInvariantLockHeld(s', j);
+  requires PerfInvariantLockInNetwork(s, j, epoch);
+  ensures PerfInvariantLockHeld(s', j, epoch);
 {
   reveal_PerfInvariantLockInNetwork();
   reveal_PerfInvariantLockHeld();
@@ -313,65 +287,65 @@ predicate PerfInvariant(tgls:TaggedGLS_State)
 {
   && TGLS_Consistency(tgls)
   && ( 
-    || (exists j :: 0 <= j < |tgls.tls.config| - 1 && PerfInvariantLockHeld(tgls, j))
-    || (exists j :: 0 < j < |tgls.tls.config| && PerfInvariantLockInNetwork(tgls, j))
+    || (exists epoch, j :: 0 <= epoch && 0 <= j < |tgls.tls.config| && PerfInvariantLockHeld(tgls, j, epoch))
+    || (exists epoch, j :: 0 <= epoch && 0 <= j < |tgls.tls.config| && PerfInvariantLockInNetwork(tgls, j, epoch))
   )
 }
 
-lemma PerfInvariantLockHeldGoesToPerfInvariant(j:int, s:TaggedGLS_State, s':TaggedGLS_State)
+lemma PerfInvariantLockHeldGoesToPerfInvariant(j:int, epoch:int, s:TaggedGLS_State, s':TaggedGLS_State)
   requires SingleGLSPerformanceAssumption(s) && TGLS_Consistency(s)
   requires SingleGLSPerformanceAssumption(s') && TGLS_Consistency(s')
   requires TGLS_Next(s, s')
   requires 0 <= j < |s.tls.config| - 1
-  requires PerfInvariantLockHeld(s, j)
+  requires PerfInvariantLockHeld(s, j, epoch)
 
   ensures PerfInvariant(s')
 {
   if !s.tls.t_environment.nextStep.LEnvStepHostIos? {
-    NotHostIos_InvLockHeldImpliesInvLockHeld(j, s, s');
+    NotHostIos_InvLockHeldImpliesInvLockHeld(j, epoch, s, s');
   } else {
     if s.tls.t_environment.nextStep.actor == s.tls.config[j] {
       if s.tls.t_environment.nextStep.nodeStep == GrantStep {
-        Grant_j_InvLockHeldImpliesInvLockInNetwork(j, s, s');
+        Grant_j_InvLockHeldImpliesInvLockInNetwork(j, epoch, s, s');
       } else {
         reveal_PerfInvariantLockHeld();
         assert false;
       }
     } else {
       if s.tls.t_environment.nextStep.nodeStep == GrantStep {
-        Grant_not_j_InvLockHeldImpliesInvLockHeld(j, s, s');
+        Grant_not_j_InvLockHeldImpliesInvLockHeld(j, epoch, s, s');
       } else {
-        Accept_not_j_InvLockHeldImpliesInvLockHeld(j, s, s');
+        Accept_not_j_InvLockHeldImpliesInvLockHeld(j, epoch, s, s');
       }
     }
   }
 }
 
-lemma PerfInvariantLockInNetworkGoesToPerfInvariant(j:int, s:TaggedGLS_State, s':TaggedGLS_State)
+lemma PerfInvariantLockInNetworkGoesToPerfInvariant(j:int, epoch:int, s:TaggedGLS_State, s':TaggedGLS_State)
   requires SingleGLSPerformanceAssumption(s) && TGLS_Consistency(s)
   requires SingleGLSPerformanceAssumption(s') && TGLS_Consistency(s')
   requires TGLS_Next(s, s')
   requires 0 < j < |s.tls.config|
-  requires PerfInvariantLockInNetwork(s, j)
+  requires PerfInvariantLockInNetwork(s, j, epoch)
 
   ensures PerfInvariant(s')
 {
   if !s.tls.t_environment.nextStep.LEnvStepHostIos? {
-    NotHostIos_InvLockInNetworkImpliesInvLockInNetwork(j, s, s');
+    NotHostIos_InvLockInNetworkImpliesInvLockInNetwork(j, epoch, s, s');
   } else {
     if s.tls.t_environment.nextStep.actor == s.tls.config[j] {
       if s.tls.t_environment.nextStep.nodeStep == GrantStep {
         reveal_PerfInvariantLockInNetwork();
         assert false;
       } else {
-        Accept_j_InvLockInNetworkImpliesInvLockHeld(j, s, s');
+        Accept_j_InvLockInNetworkImpliesInvLockHeld(j, epoch, s, s');
       }
     } else {
       if s.tls.t_environment.nextStep.nodeStep == GrantStep {
         reveal_PerfInvariantLockInNetwork();
         assert false;
       } else {
-        Accept_not_j_InvLockInNetworkImpliesInvLockInNetwork(j, s, s');
+        Accept_not_j_InvLockInNetworkImpliesInvLockInNetwork(j, epoch, s, s');
       }
     }
   }
@@ -385,13 +359,13 @@ lemma PerfInvariantMaintained(s:TaggedGLS_State, s':TaggedGLS_State)
 
   ensures PerfInvariant(s')
 {
-  if (exists j :: 0 <= j < |s.tls.config| && PerfInvariantLockHeld(s, j)) {
-    var j :| 0 <= j < |s.tls.config| - 1 && PerfInvariantLockHeld(s, j);
-    PerfInvariantLockHeldGoesToPerfInvariant(j, s, s');
+  if (exists j, epoch :: 0 <= epoch && 0 <= j < |s.tls.config| && PerfInvariantLockHeld(s, j, epoch)) {
+    var epoch, j :| 0 <= epoch && 0 <= j < |s.tls.config| && PerfInvariantLockHeld(s, j, epoch);
+    PerfInvariantLockHeldGoesToPerfInvariant(j, epoch, s, s');
   }
   else {
-    var j :| 0 < j < |s.tls.config| && PerfInvariantLockInNetwork(s, j);
-    PerfInvariantLockInNetworkGoesToPerfInvariant(j, s, s');
+    var epoch, j :| 0 <= epoch && 0 <= j < |s.tls.config| && PerfInvariantLockInNetwork(s, j, epoch);
+    PerfInvariantLockInNetworkGoesToPerfInvariant(j, epoch, s, s');
   }
 }
 
